\documentclass{article}
\setlength{\headheight}{22.50113pt}
\addtolength{\topmargin}{-10.50113pt}

\input{preamble}
\input{letterfont}
\input{macros}

\fancyhead[L]{\tbo{Josh Park \\ Prof. Shkredov}}
\fancyhead[C]{\tbo{MA 45401-H01 \\ Galois Theory Honors}}
\fancyhead[R]{\tbo{Spring 2025 \\ Homework 3}}

\begin{document}

% \begin{note}[Notation]
% In the following problems, I denote the principal ideal generated by $ f(x) $ by $ \pid{f(x)} $. \\
% In the context of a factor ring $ \fr{L}{K} $, I may use equivalence classes or coset representatives interchangeably. The meaning should be clear from context, but I will do my best to disambiguate as necessary.
% \end{note}

\setcounter{section}{3}
\setcounter{exercise}{1}
\begin{subexercise}
Show that $ t^3+t+1 $ is irreducible in $ \Ftw[t] $.
\end{subexercise}

\begin{solution}
Assume, for the sake of contradiction, that $ f(t) = t^3+t+1 $ is reducible over $ \Ftw[t] $.
Then, $ f(t) = g(t)h(t) $ for some $ g(t),h(t)\in \Ftw[t] $.
Without loss of generality, $ \deg g(t) = 2 \tand \deg h(t) = 1 $.
Since $ \deg h(t) = 1 $ over $ \Ftw[t] $, we have that either $ h(t) = t $ or $ h(t) = t+1 $.
However, notice that $ f(1) \neq 0\tand f(0)\neq 0 $.
Thus $ f(t) $ has no linear factors, contradicting that $ \deg h(t) = 1 $.
Therefore $ f(t) = t^3+t+1 $ must be irreducible over the field $ \Ftw[t] $.
\end{solution}

\begin{subexercise}
Consider the quotient ring $ L:= \fr{\Ftw[t]}{\pid{t^3+t+1}} $ and compute its size.
\end{subexercise}

\begin{solution}
Let $ f = t^3+t+1 $.

Then the factor ring $ \fr{\Ftw[t]}{\pid{f}} $ partitions elements of $ \Ftw[t] $ into the following equivalence classes: \begin{align*}
  [0],\ [1],\ [t] ,\ [t+1],\ [t\sq],\ [t\sq+1],\ [t\sq+t],\ [t\sq+t+1]
\end{align*}
Hence $ \order{L} = 8 $.
\end{solution}

\begin{subexercise}
Take $ g=t+1 $ and prove the set $ \{0,g,g^2,\ldots,g^7\} $ coincides with $ L $.
\end{subexercise}

\begin{solution}
Obviously this set has 8 elements, which agrees with our result in Exercise 3.1.2.
It remains to show that each element corresponds to a unique equivalence class from above (taken mod $ f $).
\[\begin{array}{lll}
  0   \equiv 0       &\!\!\!\!\!\!\!\!\pmod f \imp 0 \in [0] \\
  g   \equiv t+1     &\!\!\!\!\!\!\!\!\pmod f \imp g \in [t+1] \\
  g^2 \equiv t^2+1   &\!\!\!\!\!\!\!\!\pmod f \imp g^2 \in [t^2+1] \\
  g^3 \equiv t^2     &\!\!\!\!\!\!\!\!\pmod f \imp g^3 \in [t^2] \\
  g^4 \equiv t^2+t+1 &\!\!\!\!\!\!\!\!\pmod f \imp g^4 \in [t^2+t+1] \\
  g^5 \equiv t       &\!\!\!\!\!\!\!\!\pmod f \imp g^5 \in [t] \\
  g^6 \equiv t^2+t   &\!\!\!\!\!\!\!\!\pmod f \imp g^6 \in [t^2+t] \\
  g^7 \equiv 1       &\!\!\!\!\!\!\!\!\pmod f \imp g^7 \in [1]
\end{array}\]
Thus there is a clear bijection between the set $ \{0,g,g\sq,\ldots,g^7\} $ and $ L $.
\end{solution}

% \stepcounter{exercise}
\begin{exercise}
Let $K$ be a field and $p, q \in K[t]$ be irreducible polynomials over $K$, $\pid p \neq \pid q$ (this is equivalent to the statement that $p$ is coprime to $q$). Consider the field $\bbF := K(t)$ and the polynomial $g(x) = x^n + px + pq \in \bbF[x]$. Prove that $g$ is irreducible over $\bbF$.
\end{exercise}

\begin{solution}
From lecture, $ F[t] $ is a Euclidean domain for any field $ F $ and any Euclidean domain is also a unique factorization domain, so $ \bbF[x] $ is a UFD.
Next, it is easy to see that $ \gcd(g(x)) = \gcd(1, p, pq) = 1 $.
Notice that for the irreducible polynomial $ p \in \bbF $, we have that $ p \divs p $, $ p\divs pq $, $ p\ndivs 1 $ and obviously $ p\sq \ndivs pq $ (otherwise $ p\sq\divs pq \imp p\divs q $ contradicts that they are coprime).
Thus by Eisenstein's Criterion $ g $ is irreducible over $ \bbF $.
\end{solution}

\begin{exercise}
Prove that $ t^2 -7 $ is irreducible over $ \bbQ(\sqrt 5) $.
\end{exercise}

\begin{solution}
Let $ f(t) = t\sq - 7 $.
Assume for the sake of contradiction that $ f $ is reducible.
By definiton of reducible, $ f $ must equal the product of polynomials with strictly lower degree, so $ f=gh \imp \deg(g) = \deg(h) = 1 $.
This means $ g\tand h $ are linear factors, which implies that $ \exists x\in \bbQ(\sqrt 5) $ such that $ f(x) = 0 $.
Since $ x\in \bbQ(\sqrt 5) \imp x=a+b\sqrt 5$ for $ a,b\in \bbQ $, notice \begin{align*}
  f(x) = 0 &\imp (a+b\sqrt{5})\sq - 7 = 0 \\
  &\imp a\sq + 2ab\sqrt 5 + 5b\sq - 7 = 0 \\
  &\imp a\sq + 5b\sq - 7 = - 2ab\sqrt 5 \\
  &\imp \frac{a\sq + 5b\sq - 7}{-2ab} = \sqrt 5 \imp \sqrt 5\in \bbQ
\end{align*}
which is obviously a contradiction.
Thus $ f(t) = t\sq - 7 $ is irreducible over $ \bbQ(\sqrt 5) $.
\end{solution}

\stepcounter{exercise}
\begin{subexercise}
Let $ \alpha=2^{1/6} $ and $ \veps_3^3=1 $, $ \veps_3\neq 1 $. Find the minimal polynomials of $ \alpha $ over \begin{align*}
  a)\ \bbQ, \quad b)\ \bbQ(\alpha), \quad c)\ \bbQ(\alpha\sq), \quad d)\ \bbQ(\alpha\veps_3).
\end{align*}
\end{subexercise}

\begin{solution}
\begin{enumerate}[label=\alph*)]
\item In $ \bbQ $, \begin{align*}
  \alpha = 2^{1/6} &\imp x = 2^{1/6}\\
  &\imp x^6 = 2 \\
  &\imp x^6 - 2 = 0.
\end{align*}
Let $ f(x) = x^6-2 $.
By Eisenstein (using $ p=2 $), $ f $ is irreducible.
Thus $ \mu_\alpha^\bbQ (x) = x^6 - 2 $.

\item In $ \bbQ(\alpha)=\bbQ(2^{1/6}) $, \begin{align*}
  \alpha = 2^{1/6} &\imp x=2^{1/6} \\
  &\imp x - 2^{1/6} = 0.
\end{align*}
Let $ g(x) = x-2^{1/6} $.
Since $ \deg(x-2^{1/6}) = 1 $, it can not be decomposed into  polynomials of smaller degree and is therefore irreducible by definition.
Thus $ \mu_\alpha^{\bbQ(\alpha)} (x) = x - 2^{1/6} $.

\item In $ \bbQ(\alpha\sq)=\bbQ(2^{1/3}) $, \begin{align*}
  \alpha\sq = 2^{1/3} &\imp x\sq = 2^{1/3} \\
  &\imp x\sq - 2^{1/3} = 0.
\end{align*}
Let $ h(x) = x\sq-2^{1/3} $. Assuming $ h $ is reducible, it must decompose into linear factors.
However, notice $ h $ does not have any roots in $ \bbQ(2^{1/3}) $, since $ h $ only has 2 solutions by the Fundamental Theorem of Algebra, but $ \pm\alpha\not\in \bbQ(2^{1/3}) $.
Thus $ h $ can not be reduced into linear factors, whence $ \mu_\alpha^{\bbQ(\alpha^2)}(x) = x^2-2^{1/3} $.

\item Let $ \beta=\alpha\veps_3 $. In $ \bbQ(\beta) $, \begin{align*}
  \beta = \alpha\veps_3 &\imp \beta\cb = \alpha\cb \veps\cb \\
  &\imp \alpha\cb - \beta\cb = 0 \\
  &\imp x\cb - \beta\cb = 0 \\
  &\imp (x-\beta)(x\sq+\beta x + \beta\sq) = 0.
\end{align*}
Let $ p(x) = x-\beta $ and $ q(x) = x\sq+\beta x + \beta\sq $.
We know $ \alpha $ must satisfy at least one of these, but notice $ \alpha-\beta = 0 \imp \alpha = \beta $, which is obviously a contradiction since $ \beta=\alpha\veps_3 $ and $ \veps_3 \neq 1 $.
Thus $ \alpha $ satisfies $ q(x) $ and not $ p(x) $. Now, supposing $ q(x) $ is reducible, it must decompose into linear factors.
However, we can easily see that the only roots of $ q(x) $ are $ \pm \alpha$ but $ \pm\alpha\not\in \bbQ(\beta) $, otherwise $ \veps_3 \in \bbQ(\beta) $ which is obviously not true.
Therefore $ q(x) =  x\sq+\beta x + \beta\sq $ must be irreducible over $ \bbQ(\beta) = \bbQ(\alpha\veps_3) $, whence $ \mu_\alpha^{\bbQ(\alpha\veps_3)}(x) =  x\sq+\beta x + \beta\sq = x\sq+\alpha\veps_3x + \alpha\sq\veps_3\sq$.
\end{enumerate}
\end{solution}

\begin{subexercise}
In each case (a---d), find the conjugate elements of all roots of $ x^6-2 $.
\end{subexercise}

\begin{solution}
\begin{enumerate}[label=\alph*)]
  \item In $ \bbQ $, we have that $ \mu_\alpha^{\bbQ}(x) = x^6-2 $.
  By the Fundamental Theorem of Algebra, this equation has 6 solutions.
  Thus, the conjugates of $ \alpha $ over $ \bbQ $ are $ \{\alpha\veps_6^k \st 0\leq k < 6 \} $, where $ \veps_6 = \exp(\frac{i\pi}{3}) = \frac{1}{2}+\frac{i\sqrt 3}{2} $.

  \item In $ \bbQ(\alpha) $, we have that $ \mu_\alpha^{\bbQ(\alpha)}(x) =  x - 2^{1/6} $.
  By FTA, this equation only has one solution.
  Thus the sole conjuage of $ \alpha $ over $ \bbQ(\alpha) $ is itself, $ \alpha $.

  \item In $ \bbQ(\alpha\sq) $, we have that $ \mu_\alpha^{\bbQ(\alpha\sq)}(x) = x^2-2^{1/3} $.
  By FTA, this equation has 2 solutions.
  It is trivial to see that the conjuates of $ \alpha $ over $ \bbQ(\alpha\sq) $ are $ \pm\alpha $.

  \item In $ \bbQ(\alpha\veps_3) $, we have that $ \mu_\alpha^{\bbQ(\alpha\veps_3)}(x) = x\sq+\alpha\veps_3x + \alpha\sq\veps\sq $.
  By FTA, this equation has 2 solutions.
  We know that one solution to this equation is $ x_1 = \alpha $, so by Vieta's formulae we have $ x_2 = -\alpha\veps_3 - \alpha = -\alpha(\veps_3+1) $.
  Notice that $ \veps_3^3 = 1 \imp \veps_3^3-1=0 $.
  We know $ \veps_3\neq 1 $, so we can factor out the linear term for which the solution is 1.
  That is, $ \veps_3^3-1 = (\veps_3-1)(\veps_3\sq+\veps_3+1) $.
  So our root of unity must satisfy $ \veps_3\sq+\veps_3+1 = 0 \imp \veps_3\sq=-(\veps_3+1) $.
  Thus we can substitute this into our previous equation to find $ x_2 = \alpha\veps_3\sq $, whence our algebraic conjugates of $ \alpha $ are $ \alpha, \alpha\veps_3\sq $.
\end{enumerate}
\end{solution}

\end{document}
