\documentclass[a4paper]{article}

\input{preamble}
\input{letterfont}
\input{macros}

\begin{document}
\section{Final remarks I}
\begin{tdefinition}[Sylvester matrix]

\end{tdefinition}

\begin{tdefinition}[Resultant]

\end{tdefinition}

\begin{ttheorem}
  Let \( \alpha_i \) be roots of \( f \) and \( \beta_j \) be roots of \( g \).
  Then \begin{align*}
    R(f,g) &= a_0^m b_0^n \prod_i(\alpha_i-\beta_j) \\
    &= a_0^m \prod_i g(\alpha_i) = b_0^n \prod_i f(\beta_i)
  \end{align*} \hl{R?}
\end{ttheorem}

\begin{tcorollary}
  \begin{enumerate}
    \item \( R(f,g) = (-1)^{\deg f \cdot \deg g}R(g,f) \)
    \item If \( f = gq + r \imp R(f,g) = b_0^{\deg f - \deg R} R(r,g) \)
    \item \( R(f,gh) = R(f,g)R(f,h) \)
  \end{enumerate}
\end{tcorollary}

\begin{tcorollary}
  Let \( f(t) = a_0 t^{n} + \cdots + a_n,\ a_0\neq 0 \).
  Then \( R(f,f') = (-1)^{\frac{n(n-1)}{2}}\prod_{i<j}(\alpha_i-\alpha_j)\sq \)
\end{tcorollary}

\end{document}